Add basic blockchain structures & axioms

Core/Blockchain.v
@@ -8,10 +8,74 @@ Unset Strict Implicit.
 Unset Printing Implicit Defensive.
 
 (* A fomalization of a blockchain structure *)
+Definition Hash := nat.
+Definition VProof := nat.
+Definition Transaction := nat.
 
-(* The first approximation: a number of axioms *)
+Record Block :=
+  mkB {
+    prevBlockHash : Hash;
+    txs : seq Transaction;
+    proof : VProof;
+  }.
 
-(* TODO: formalize the blocktree *)
+Parameter hashB : Block -> Hash.
+Definition eq_block b b' := hashB b == hashB b'.
 
-(* TODO: formalize the blockchain *)
+Definition Blockchain := seq Block.
 
+(* We might want to introduce a notion of time *)
+Parameter VAF : VProof -> Blockchain -> bool.
+Parameter blockValid : Block -> Blockchain -> bool.
+
+Parameter CFR_gt : Blockchain -> Blockchain -> bool.
+Notation "A > B" := (CFR_gt A B).
+
+Definition BlockTree := seq Block.
+
+Parameter btExtend : BlockTree -> Block -> BlockTree.
+Parameter btChain : BlockTree -> Blockchain.
+
+(* Axioms *)
+Axiom hashB_inj : forall (b b': Block), hashB b == hashB b' -> b = b'.
+
+Module BlockEq.
+Lemma eq_blockP : Equality.axiom eq_block.
+Proof.
+move=> b b'. rewrite/eq_block. apply: (iffP idP).
+  - by apply: hashB_inj.
+  - move=> eq. by rewrite eq.
+Qed.
+
+Canonical Block_eqMixin := Eval hnf in EqMixin eq_blockP.
+Canonical Block_eqType := Eval hnf in EqType Block Block_eqMixin.
+End BlockEq.
+Export BlockEq.
+
+Axiom blockValid_imp_VAF :
+  forall (b : Block) (bc : Blockchain),
+    (blockValid b bc) -> (VAF (proof b) bc).
+
+(* TODO: justify the need for this *)
+Axiom no_proof_reuse :
+  forall (b b' : Block) (bc : Blockchain),
+    b <> b' -> (blockValid b bc) -> (blockValid b' bc) ->
+    (proof b) <> (proof b').
+
+Axiom CFR_strictly_increases :
+  forall (bc : Blockchain) (b : Block),
+    blockValid b bc -> (bc ++ [:: b]) > bc.
+
+Axiom btExtend_preserve :
+  forall (bt : BlockTree) (ob b : Block), let: bt' := btExtend bt b in
+    ob \in bt -> ob \in bt'.
+
+Axiom btExtend_withDup_noEffect :
+  forall (bt : BlockTree) (b : Block), let: bt' := btExtend bt b in
+    b \in bt -> bt = bt'.
+
+(* TODO: explain *)
+Axiom btExtend_withNew_sameOrBetter :
+  forall (bt : BlockTree) (b : Block), let: bt' := btExtend bt b in
+    b \notin bt ->
+      (b \in (btChain bt') <-> (btChain bt') > (btChain bt)).
